theories/Infra/MoreTac.v
@@ -1,7 +1,7 @@
 Ltac let_unfold id :=
   cbv beta delta [id];
   repeat match goal with
-         | [ |- context [ let s := ?e in _ ] ] => set (s:=e)
+         | [ |- context [ let s := ?e in _ ] ] => set (s:=e) in *
          | [ |- context [let (a, b) := ?e in _] ] =>
            let a := fresh a in let b := fresh b in case_eq e; intros b a ?
          | [ H : ?x = (?s, ?t) |- _ ] =>
@@ -12,6 +12,17 @@ Ltac let_unfold id :=
              let s := eval cbv beta in (t s) in
                  let x := context f[s] in
                  change x
+         end.
+
+Ltac let_unfold' id H :=
+  cbv beta delta [id] in H;
+  repeat match type of H with
+         | context [ let s := ?e in _ ] => set (s:=e) in *
+         | context f [ let s := ?e in @?t s ] =>
+           is_var e;
+             let s := eval cbv beta in (t s) in
+                 let x := context f[s] in
+                 change x in H
          end.
 
 Tactic Notation "refold" :=
